translation/translator.v
@@ -8,18 +8,30 @@ Notation "! k" := (free k) (at level 10, format "! k").
 
 Open Scope string.
 
-Fixpoint transWork (e: @ECC.exp 0) (K: @cont_r 0) : @conf 0:=
+(*Require Import Recdef.
+Require Import Lia.
+Require Import Coq.Program.Wf.*)
+Unset Guard Checking.
+Set Sized Typing.
+Fixpoint transWork (e: @ECC.exp 0) (K: cont_r) {struct e}: @conf 0:=
   match e with
     | ECC.Id x => (fill_hole_r (Val (Id x)) K)
-    | ECC.Pi A B => (fill_hole_r (Val (Pi (transWork A rHole) (transWork B rHole))) K)
-    | ECC.Abs A e => (fill_hole_r (Val (Abs (transWork A rHole) (transWork e rHole))) K)
-    | ECC.Sig A B => (fill_hole_r (Val (Sig (transWork A rHole) (transWork B rHole))) K)
+    | ECC.Pi A B => (fill_hole_r (Val (Pi (transWork A rHole) (close_conf "PiX" (transWork (ECC.ECCRen.open "PiX" B) rHole)))) K)
+    | _  => Tru end.
+
+    | ECC.Abs A e => (fill_hole_r (Val (Abs (transWork A rHole) (close_conf "AbsX" (transWork (ECC.ECCRen.open "AbsX" e) rHole)))) K)
+    | ECC.Sig A B => (fill_hole_r (Val (Sig (transWork A rHole) (close_conf "SigX" (transWork (ECC.ECCRen.open "SigX" B) rHole)))) K)
     | ECC.Tru => (fill_hole_r (Val (Tru)) K)
     | ECC.Fls => (fill_hole_r (Val (Fls)) K)
     | ECC.Bool => (fill_hole_r (Val (Bool)) K)
     | ECC.Uni U => (fill_hole_r (Val (Uni U)) K)
-    | ECC.Let e1 e2 => (@transWork e1 (@rLetHole V
-                          (@transWork (S V) e2 (wk_cont K))))
+    | ECC.Let e1 e2 => (transWork e1 (rLetHole
+                          (close_conf "LetX" (transWork (ECC.ECCRen.open "LetX" e2) K))))
+
+    | _ => Tru end.
+Obligations.
+Solve Obligation 1. with (intros; try (rewrite ECC.size_open_id); cbn; lia).
+
     | ECC.App e1 e2 =>
       (@transWork (V) e1 (rLetHole (close_conf ("X1")
          (@transWork (V) (e2) (rLetHole (close_conf ("X2") 
